packages/zoe/spec/jessie_module.v
@@ -36,7 +36,7 @@ Module JessieModule.
 
   Definition init_state (imports : list (string * val)) : state :=
     State (st_next_loc empty_state) (st_store empty_state) (st_frozen empty_state)
-      (imports ++ st_env empty_state).
+      (imports ++ st_env empty_state) (st_cells empty_state) (st_dyn_prims empty_state).
 
   Fixpoint eval_decls (fuel : nat) (σ : state) (decls : list module_decl)
       : option (exports * state) :=
@@ -48,7 +48,7 @@ Module JessieModule.
         | CoreLit v =>
             match eval_decls fuel
                 (State (st_next_loc σ1) (st_store σ1) (st_frozen σ1)
-                  ((name, v) :: st_env σ1))
+                  ((name, v) :: st_env σ1) (st_cells σ1) (st_dyn_prims σ1))
                 decls' with
             | Some (outs, σ2) => Some ((name, v) :: outs, σ2)
             | None => None
